
Module 4:Lecture notes

By Dr. Keya Doshi

Successive Differentiation

Definition

If a function is differentiated once and if derivative of a function differentiated again and again with respect to same independent variable then such process is known as **Successive Differentiation** of a function

i.e. If $y = f(x)$ is a differentiable function of x then

$$\begin{aligned}y_1 &= \frac{dy}{dx} \\ \Rightarrow y_2 &= \frac{d}{dx} \left(\frac{dy}{dx} \right) = \frac{d^2y}{dx^2} \\ \Rightarrow y_3 &= \frac{d}{dx} \left(\frac{d^2y}{dx^2} \right) = \frac{d^3y}{dx^3}\end{aligned}$$

Continuing this process we have

$$y_n = \frac{d}{dx} \left(\frac{d^{n-1}y}{dx^{n-1}} \right) = \frac{d^n y}{dx^n}$$

are called successive n^{th} derivatives of y and are denoted by $y_n, f^{(n)}(x), \frac{d^n}{dx^n}$ and the values of this derivatives at an arbitrary point a is denoted by $[y_n]_{(a)}, f^{(n)}(a), \left[\frac{d^n y}{dx^n} \right]_{x=a}$

n^{th} derivatives of Algebraic Functions

Case(1)

If $y = (ax + b)^m$ then

$$y_n = m(m-1)(m-2)\dots(m-n+1)a^n(ax+b)^{(m-n)} \quad n < m$$

Proof

Let

$$\begin{aligned}y &= (ax + b)^m \\ \Rightarrow y_1 &= m(ax + b)^{(m-1)}a \\ \Rightarrow y_2 &= m(m-1)(ax + b)^{(m-2)}a^2 \\ \Rightarrow y_3 &= m(m-1)(m-2)(ax + b)^{(m-3)}a^3\end{aligned}$$

Continuing differentiation upto n^{th} derivatives, we have

$$y_n = m(m-1)(m-2)....(m-(n-1))(ax+b)^{(m-n)}a^n$$

$$y_n = m(m-1)(m-2)....(m-n+1)(ax+b)^{(m-n)}a^n....(1)$$

This holds true for positive integer m and $n < m$ Multiplying and dividing result (1) by $(m-n)(m-n-1)...$ 3.2.1 we have

$$y_n = \frac{m!}{(m-n)!}(ax+b)^{(m-n)}a^n....(2)$$

If $n = m$ then from above result

$$y_n = n!a^n....(3)$$

This holds true for positive integer m and $n < m$ **Case(2)**

If $y = (ax+b)^{(-m)}$ then

$$y_n = \frac{(-1)^n(m+n-1)!a^n}{(m-1)!(ax+b)^{(m+n)}}$$

Proof

If m is negative real integer then let $m = -p$ where p is positive integer, then

$$y = \frac{1}{(ax+b)^m} \implies y = (ax+b)^{(-m)}$$

Then by(1)

$$y_n = (-m)(-m-1)(-m-2)....(-m-n+1)(ax+b)^{(-m-n)}a^n$$

$$y_n = (-1)^nm(m-1)(m-2)....(m+n-1)(ax+b)^{-(m+n)}a^n$$

$$y_n = \frac{(-1)^n(m+n-1)!(ax+b)^{-(m+n)}a^n}{(m-1)!}$$

(Multiplying and dividing by $(m-1)(m-2)...$ 3.2.1 and simplifying)

Hence for negative integer m i.e. for $y = \frac{1}{(ax+b)^m}$

$$y_n = \frac{(-1)^n(m+n-1)!a^n}{(m-1)!(ax+b)^{(m+n)}}$$

Case(3)

If $y = \log_e(ax + b)$ then

$$y_n = \frac{(-1)^{n-1}(n-1)!a^n}{(ax+b)^n}$$

Proof

Let

$$\begin{aligned} y &= \log_e(ax + b) \\ \Rightarrow y_1 &= \frac{1}{ax+b}a \\ \Rightarrow y_2 &= \frac{(-1)}{(ax+b)^2}a^2 \\ \Rightarrow y_3 &= \frac{(-1)(-2)}{(ax+b)^3}a^3 \end{aligned}$$

Continuing differentiation upto n^{th} derivatives, we have

$$\begin{aligned} y_n &= \frac{(-1)(-2)\dots(-n+1)}{(ax+b)^n}a^n \\ y_n &= \frac{(-1)^{(n-1)}(n-1)!a^n}{(ax+b)^n} \dots (1) \end{aligned}$$

Case(4)

If $y = a^{(bx+c)}$ then

$$y_n = b^n (\log_e a)^n a^{bx+c}$$

Proof

Let

$$\begin{aligned} y &= a^{(bx+c)} \\ \Rightarrow y_1 &= a^{(bx+c)} \log_e a \cdot b \\ \Rightarrow y_2 &= a^{(bx+c)} (\log_e a)^2 b^2 \\ \Rightarrow y_3 &= a^{(bx+c)} (\log_e a)^3 b^3 \end{aligned}$$

Continuing differentiation upto n^{th} derivatives, we have

$$y_n = a^{(bx+c)} (\log_e a)^n b^n \dots (1)$$

n^{th} derivatives of Trigonometric Functions

Case(1)

If $y = \sin(ax + b)$ then

$$y_n = a^n \sin\left(ax + b + \frac{n\pi}{2}\right)$$

Proof 1

Let

$$\begin{aligned} y &= \sin(ax + b) \\ \Rightarrow y_1 &= a \cos(ax + b) \\ &= a \sin\left(ax + b + \frac{\pi}{2}\right) \\ \Rightarrow y_2 &= a^2 \cos\left(ax + b + \frac{\pi}{2}\right) \\ &= a^2 \sin\left(ax + b + \frac{\pi}{2} + \frac{\pi}{2}\right) \\ &= a^2 \sin(ax + b + \pi) \\ \Rightarrow y_3 &= a^3 \cos\left(ax + b + \frac{2\pi}{2}\right) \\ &= a^3 \sin\left(ax + b + \frac{2\pi}{2} + \frac{\pi}{2}\right) \\ &= a^3 \sin\left(ax + b + \frac{3\pi}{2}\right) \end{aligned}$$

Continuing differentiation upto n^{th} derivatives, we have

$$\begin{aligned} y_n &= \frac{d^n}{dx^n} [\sin(ax + b)] \\ y_n &= a^n \sin\left(ax + b + \frac{n\pi}{2}\right) \dots (1) \end{aligned}$$

Case(2)

If $y = \cos(ax + b)$ then

$$y_n = a^n \cos\left(ax + b + \frac{n\pi}{2}\right)$$

Proof 2

Let

$$\begin{aligned} y &= \cos(ax + b) \\ \Rightarrow y_1 &= -a \sin(ax + b) \\ &= a \cos\left(ax + b + \frac{\pi}{2}\right) \\ \Rightarrow y_2 &= -a^2 \sin\left(ax + b + \frac{\pi}{2}\right) \\ &= a^2 \cos\left(ax + b + \frac{\pi}{2} + \frac{\pi}{2}\right) \\ &= a^2 \cos(ax + b + \pi) \\ \Rightarrow y_3 &= -a^3 \sin\left(ax + b + \frac{2\pi}{2}\right) \\ &= a^3 \cos\left(ax + b + \frac{2\pi}{2} + \frac{\pi}{2}\right) \\ &= a^3 \cos\left(ax + b + \frac{3\pi}{2}\right) \end{aligned}$$

Continuing differentiation upto n^{th} derivatives, we have

$$\begin{aligned} y_n &= \frac{d^n}{dx^n} [\cos(ax + b)] \\ y_n &= a^n \cos\left(ax + b + \frac{n\pi}{2}\right) \dots (2) \end{aligned}$$

Special Cases

Case(1)

If $y = e^{ax} \sin(bx + c)$ then

$$y_n = (a^2 + b^2)^{\frac{n}{2}} e^{ax} \sin\left[bx + c + n \tan^{-1}\left(\frac{b}{a}\right)\right]$$

Proof

Let

$$\begin{aligned}
 y &= e^{ax} \sin(bx + c) \\
 \implies y_1 &= a e^{ax} \sin(bx + c) + e^{ax} b \cos(bx + c) \\
 &= e^{ax} [a \sin(bx + c) + b \cos(bx + c)] \dots (1)
 \end{aligned}$$

Let $a = r \cos \theta$ and $b = r \sin \theta$

Then $r = (a^2 + b^2)^{\frac{1}{2}}$ and $\theta = \tan^{-1} \left(\frac{b}{a} \right)$

Substituting in (1), we have

$$\begin{aligned}
 y_1 &= e^{ax} [a \sin(bx + c) + b \cos(bx + c)] \\
 &= e^{ax} [(r \cos \theta) \sin(bx + c) + (r \sin \theta) \cos(bx + c)] \\
 &= r e^{ax} [\sin(bx + c) \cos \theta + \cos(bx + c) \sin \theta] \\
 y_1 &= r e^{ax} [\sin(bx + c + \theta)]
 \end{aligned}$$

Again differentiating in the same manner

$$\begin{aligned}
 y_1 &= r e^{ax} [\sin(bx + c + \theta)] \\
 \implies y_2 &= r [a e^{ax} (\sin(bx + c + \theta)) + r (b e^{ax} \cos(bx + c + \theta))] \\
 &= r e^{ax} [a \sin(bx + c + \theta) + b \cos(bx + c + \theta)] \\
 &= r e^{ax} [r \cos \theta \sin(bx + c + \theta) + r \sin \theta \cos(bx + c + \theta)] \\
 &= r^2 e^{ax} [\sin(bx + c + \theta) \cos \theta + \cos(bx + c + \theta) \sin \theta] \\
 &= r^2 e^{ax} [\sin(bx + c + \theta + \theta)] \\
 y_2 &= r^2 e^{ax} [\sin(bx + c + 2\theta)]
 \end{aligned}$$

Continuing differentiation upto n^{th} derivatives, we have

$$\begin{aligned}
 y_n &= r^n e^{ax} [\sin(bx + c + n\theta)] \\
 y_n &= (a^2 + b^2)^{\frac{n}{2}} e^{ax} \sin \left[bx + c + n \tan^{-1} \left(\frac{b}{a} \right) \right]
 \end{aligned}$$

Case(2)

If $y = e^{ax} \cos(bx + c)$ then

$$y_n = (a^2 + b^2)^{\frac{n}{2}} e^{ax} \cos \left[bx + c + n \tan^{-1} \left(\frac{b}{a} \right) \right]$$

Proof

Let

$$\begin{aligned} y &= e^{ax} \cos(bx + c) \\ \implies y_1 &= a e^{ax} \cos(bx + c) - e^{ax} b \sin(bx + c) \\ &= e^{ax} [a \cos(bx + c) - b \sin(bx + c)] \dots (1) \end{aligned}$$

Let $a = r \cos \theta$ and $b = r \sin \theta$

Then $r = (a^2 + b^2)^{\frac{1}{2}}$ and $\theta = \tan^{-1} \left(\frac{b}{a} \right)$

Substituting in (1), we have

$$\begin{aligned} y_1 &= e^{ax} [a \cos(bx + c) - b \sin(bx + c)] \\ &= e^{ax} [(r \cos \theta) \cos(bx + c) - (r \sin \theta) \sin(bx + c)] \\ &= r e^{ax} [\cos(bx + c) \cos \theta - \sin(bx + c) \sin \theta] \\ y_1 &= r e^{ax} [\cos(bx + c + \theta)] \end{aligned}$$

Again differentiating in the same manner

$$\begin{aligned} y_1 &= r e^{ax} [\cos(bx + c + \theta)] \\ \implies y_2 &= r [a e^{ax} (\cos(bx + c + \theta)) - r (b e^{ax} \sin(bx + c + \theta))] \\ &= r e^{ax} [a \cos(bx + c + \theta) - b \sin(bx + c + \theta)] \\ &= r e^{ax} [r \cos \theta \cos(bx + c + \theta) - r \sin \theta \sin(bx + c + \theta)] \\ &= r^2 e^{ax} [\cos(bx + c + \theta) \cos \theta - \sin(bx + c + \theta) \sin \theta] \\ &= r^2 e^{ax} [\cos(bx + c + \theta + \theta)] \\ y_2 &= r^2 e^{ax} [\cos(bx + c + 2\theta)] \end{aligned}$$

Continuing differentiation upto n^{th} derivatives, we have

$$\begin{aligned} y_n &= r^n e^{ax} [\cos(bx + c + n\theta)] \\ y_n &= (a^2 + b^2)^{\frac{n}{2}} e^{ax} \cos \left[bx + c + n \tan^{-1} \left(\frac{b}{a} \right) \right] \end{aligned}$$

Examples

Example 1

Find n^{th} derivatives of following functions

$$y = \frac{x+3}{(x-1)(x+2)}$$

Solution

Given

$$y = \frac{x+3}{(x-1)(x+2)}$$
$$y = \frac{A}{(x-1)} + \frac{B}{(x+2)} \dots (1)$$

Using Partial fraction method, let

$$x+3 = A(x+2) + B(x-1)$$

$$\text{For } x = 1 ; 4 = A(3) \implies A = \frac{4}{3}$$

$$x = -2 ; 1 = B(-3) \implies B = \frac{-1}{3}$$

Substituting in (1)

$$y = \frac{A}{(x-1)} + \frac{B}{(x+2)}$$

$$y = \frac{\frac{4}{3}}{(x-1)} + \frac{\frac{-1}{3}}{(x+2)}$$

Taking n^{th} derivative

$$\begin{aligned}
\frac{d^n}{dx^n} [y] &= \frac{d^n}{dx^n} \left[\frac{\frac{4}{3}}{(x-1)} \right] + \frac{d^n}{dx^n} \left[\frac{\frac{-1}{3}}{(x+2)} \right] \\
&= \frac{4}{3} \frac{d^n}{dx^n} \left[\frac{1}{(x-1)} \right] - \frac{1}{3} \frac{d^n}{dx^n} \left[\frac{1}{(x+2)} \right] \\
&= \frac{4}{3} \left[\frac{(-1)^n n!}{(x-1)^{n+1}} \right] - \frac{1}{3} \left[\frac{(-1)^n n!}{(x+2)^{n+1}} \right] \\
y_n &= \frac{(-1)^n n!}{3} \left[\frac{4}{(x-1)^{n+1}} - \frac{1}{(x+2)^{n+1}} \right]
\end{aligned}$$

Example 2

If $y = x \log \left(\frac{x-1}{x+1} \right)$ then prove that

$$y_n = (-1)^{n-2} (n-2)! \left[\frac{x-n}{(x-1)^n} - \frac{x+n}{(x+1)^n} \right]$$

Solution

Given

$$\begin{aligned}
y &= x \log \left(\frac{x-1}{x+1} \right) \\
\Rightarrow y &= x \log (x-1) - x \log (x+1) \\
\Rightarrow y_1 &= \log (x-1) - \log (x+1) + \frac{x}{x-1} - \frac{x}{x+1} \\
\Rightarrow y_1 &= \log (x-1) - \log (x+1) + 1 + \frac{1}{x-1} - 1 + \frac{1}{x+1} \\
\Rightarrow y_1 &= \log (x-1) - \log (x+1) + \frac{1}{x-1} + \frac{1}{x+1}
\end{aligned}$$

Taking n^{th} derivative of y , i.e. taking $(n-1)^{th}$ derivative of y_1

$$\begin{aligned}
\frac{d^n}{dx^n} [y] &= \frac{d^{n-1}}{dx^{n-1}} \left[\log(x-1) - \log(x+1) + \frac{1}{x-1} + \frac{1}{x+1} \right] \\
&= \frac{d^{n-1}}{dx^{n-1}} [\log(x-1)] - \frac{d^{n-1}}{dx^{n-1}} [\log(x+1)] + \\
&\quad \frac{d^{n-1}}{dx^{n-1}} \left[\frac{1}{x-1} \right] + \frac{d^{n-1}}{dx^{n-1}} \left[\frac{1}{x+1} \right] \\
&= \frac{(-1)^{n-2}(n-2)!}{(x-1)^{n-1}} - \frac{(-1)^{n-2}(n-2)!}{(x+1)^{n-1}} + \frac{(-1)^{n-1}(n-1)!}{(x-1)^n} + \\
&\quad \frac{(-1)^{n-1}(n-1)!}{(x+1)^n}
\end{aligned}$$

$$y_n = (-1)^{n-2}(n-2)! \left[\frac{x-1}{(x-1)^n} - \frac{x+1}{(x+1)^n} + \frac{-n+1}{(x-1)^n} + \frac{-n+1}{(x+1)^n} \right]$$

$$y_n = (-1)^{n-2}(n-2)! \left[\frac{x-n}{(x-1)^n} - \frac{x+n}{(x+1)^n} \right]$$

Example 3

If

$$y = \sin^2 x \cos^3 x$$

then find y_n **Solution**

Given

$$\begin{aligned}
 y &= \sin^2 x \cos^3 x \\
 \implies y &= \sin^2 x \cos^2 x \cos x \\
 \implies y &= \frac{1}{4} (2\sin^2 x \cos^2 x)^2 \cos x \\
 \implies y &= \frac{1}{4} (\sin 2x)^2 \cos x \\
 \implies y &= \frac{1}{8} (2\sin^2 2x) \cos x \\
 \implies y &= \frac{1}{8} (1 - \cos 4x) \cos x \\
 \implies y &= \frac{1}{8} (\cos x - \cos 4x \cos x) \\
 \implies y &= \frac{1}{16} (2\cos x - 2 \cos 4x \cos x) \\
 \implies y &= \frac{1}{16} (2\cos x - \cos 5x - \cos 3x)
 \end{aligned}$$

Taking n^{th} derivative of y

$$y_n = \frac{1}{16} \left[2 \cos \left(x + \frac{n\pi}{2} \right) - 5^n \cos \left(5x + \frac{n\pi}{2} \right) - 3^n \cos \left(3x + \frac{n\pi}{2} \right) \right]$$

$$y_n = \frac{1}{8} \cos \left(x + \frac{n\pi}{2} \right) - \frac{5^n}{16} \cos \left(5x + \frac{n\pi}{2} \right) - \frac{3^n}{16} \cos \left(3x + \frac{n\pi}{2} \right)$$

Liebnitz theorem

Statement

If u and v are two functions of x with u_n and v_n be their n^{th} derivatives, then n^{th} derivative of their product uv is given by

$$(uv)_n = {}^nC_0 u_n v + {}^nC_1 u_{n-1} v_1 + \dots + {}^nC_r u_{n-r} v_r + \dots + {}^nC_n u v_n$$

NOTE:

1) $(uv)_n = (vu)_n$

2) Function whose n^{th} derivative is known is considered as u

Example(Type 1)

Find n^{th} derivative of

1) $x \sin 3x$ 2) $x^2 e^{ax}$

Solution

(1) Given $y = x \sin 3x$

Let $u = \sin 3x$ and $v = x$

By Liebnitz Rule

$$(uv)_n = {}^nC_0 u_n v + {}^nC_1 u_{n-1} v_1 + \dots + {}^nC_r u_{n-r} v_r + \dots + {}^nC_n u v_n \dots \textbf{(1)}$$

Now $u = \sin 3x \implies u_n = 3^n \sin(3x + \frac{n\pi}{2})$

and $v = x \implies v_1 = 1$ and $v_n = 0 \quad n \geq 2$

Substituting in (1), we have

$$(x \sin 3x)_n = x 3^n \sin(3x + \frac{n\pi}{2}) + n 1 3^{n-1} \sin(3x + \frac{(n-1)\pi}{2})$$

$$(x \sin 3x)_n = 3^{n-1} \left[3x \sin(3x + \frac{n\pi}{2}) + n \sin(3x + \frac{(n-1)\pi}{2}) \right]$$

(2) Given $y = x^2 e^{ax}$

Let $u = e^{ax}$ and $v = x^2$

By Liebnitz Rule

$$(uv)_n = {}^nC_0 u_n v + {}^nC_1 u_{n-1} v_1 + \dots + {}^nC_r u_{n-r} v_r + \dots + {}^nC_n u v_n$$

$$(x^2 e^{ax})_n = x^2 a^n e^{ax} + n 2x a^{n-1} e^{ax} + \frac{n(n-1)}{2!} 2 a^{n-2} e^{ax}$$

$$(x^2 e^{ax})_n = a^n e^{ax} \left[x^2 + \frac{2n}{a}x + \frac{n(n-1)}{a^2} \right]$$

Example(Type 2)

If $y = \frac{\log x}{x}$ Prove that

$$y_5 = \frac{5!}{x^6} \left[1 + \frac{1}{2} + \frac{1}{3} + \frac{1}{4} + \frac{1}{5} - \log x \right]$$

Solution

Given $y = \frac{\log x}{x} = \frac{1}{x} \log x$

Let $u = \frac{1}{x}$ and $v = \log x$

Now

$$u = \frac{1}{x}$$

$$\Rightarrow u_n = \frac{(-1)^n n!}{x^{n+1}}$$

and

$$v = \log x$$

$$\Rightarrow v_n = \frac{(-1)^{n-1} (n-1)!}{x^n}$$

By Liebnitz Rule

$$(uv)_n = {}^nC_0 u_n v + {}^nC_1 u_{n-1} v_1 + \dots + {}^nC_r u_{n-r} v_r + \dots + {}^nC_n uv_n$$

$$\begin{aligned} \left(\frac{1}{x} \log x\right)_n &= \left(\frac{(-1)^n n!}{x^{n+1}}\right) \log x + n \left(\frac{(-1)^{n-1} (n-1)!}{x^n}\right) \frac{1}{x} + \frac{n(n-1)}{2!} \left(\frac{(-1)^{n-2} (n-2)!}{x^{n-1}}\right) \frac{-1}{x^2} \\ &+ \frac{1}{x} \left(\frac{(-1)^{n-1} (n-1)!}{x^n}\right) \end{aligned}$$

$$y_n = \left(\frac{1}{x} \log x\right)_n = \frac{(-1)^n n!}{x^{n+1}} \left[\log x - \left(1 + \frac{1}{2} + \frac{1}{3} + \dots + \frac{1}{n}\right) \right]$$

For $n = 5$

$$y_5 = \frac{-5!}{x^6} \left[\log x - \left(1 + \frac{1}{2} + \frac{1}{3} + \frac{1}{5}\right) \right]$$

$$y_5 = \frac{5!}{x^6} \left[\left(1 + \frac{1}{2} + \frac{1}{3} + \frac{1}{5}\right) - \log x \right]$$

Example(Type 3)

If $\log y = \tan^{-1} x$ Prove that

$$(1+x^2)y_{n+2} - [2(n+1)x - 1]y_{n+1} + n(n+1)y_n = 0$$

Solution

Given

$$\begin{aligned}
 \log y &= \tan^{-1} x \\
 \implies y &= e^{\tan^{-1} x} \\
 \implies y_1 &= e^{\tan^{-1} x} \left(\frac{1}{1+x^2} \right) \\
 \implies (1+x^2)y_1 &= e^{\tan^{-1} x} = y
 \end{aligned}$$

again differentiating

$$(1+x^2)y_2 + 2x y_1 = y_1$$

$$(1+x^2)y_2 + (2x-1) y_1 = 0 \dots (1)$$

Differentiating (1) n^{th} time using Liebnitz Rule

$$\left[(1+x^2)y_{n+2} + n(2x)y_{n+1} + \frac{n(n-1)}{2!} 2y_n \right] + [(2x-1)y_{n+1} + n(2)y_n] = 0$$

$$\implies (1+x^2)y_{n+2} + (2nx+2x-1)y_{n+1} + (n^2-n+2n)y_n = 0$$

$$\implies (1+x^2)y_{n+2} + [2(n+1)-1]y_{n+1} + n(n+1)y_n = 0$$

Hence Proved

Example(Type 3)

If $y^{\frac{1}{m}} + y^{-\frac{1}{m}} = 2x$ Prove that

$$(x^2-1)y_{n+2} + 2(n+1)xy_{n+1} + (n^2-m^2)y_n = 0$$

Solution

Given

$$\begin{aligned}
y^{\frac{1}{m}} + y^{-\frac{1}{m}} &= 2x \\
\therefore y^{\frac{2}{m}} + 1 &= 2xy^{\frac{1}{m}} \\
\therefore \left(y^{\frac{1}{m}}\right)^2 - 2xy^{\frac{1}{m}} + 1 &= 0 \\
\therefore y^{\frac{1}{m}} &= \frac{-(-2x) \pm \sqrt{4x^2 - 4}}{2} \\
&= \frac{(2x) \pm 2\sqrt{x^2 - 1}}{2} \\
\therefore y^{\frac{1}{m}} &= x \pm \sqrt{x^2 - 1} \\
\therefore y &= (x \pm \sqrt{x^2 - 1})^m
\end{aligned}$$

Considering

$$\begin{aligned}
y &= (x + \sqrt{x^2 - 1})^m \\
\implies y_1 &= m(x + \sqrt{x^2 - 1})^{m-1} \left[1 + \frac{2x}{2\sqrt{x^2 - 1}} \right] \\
\implies y_1 &= m(x + \sqrt{x^2 - 1})^{m-1} \left[\frac{x + \sqrt{x^2 - 1}}{\sqrt{x^2 - 1}} \right] \\
\implies \sqrt{x^2 - 1} y_1 &= m(x + \sqrt{x^2 - 1})^m \\
\implies \sqrt{x^2 - 1} y_1 &= m y \\
\implies (x^2 - 1) y_1^2 &= m^2 y^2
\end{aligned}$$

Differentiating w.r.t x

$$\begin{aligned}
(x^2 - 1) 2y_1 y_2 + (2x)y_1^2 &= 2 m^2 y y_1 \\
(x^2 - 1) y_2 + xy_1 - m^2 y &= 0 \dots (1)
\end{aligned}$$

Differentiating (1) n^{th} time using Liebnitz Rule

$$\begin{aligned}
\left[(x^2 - 1)y_{n+2} + n(2x)y_{n+1} + \frac{n(n-1)}{2!}2y_n \right] + [xy_{n+1} + ny_n] - m^2 y_n &= 0 \\
\implies (x^2 - 1)y_{n+2} + (2nx + x)y_{n+1} + (n^2 - n + n - m^2)y_n &= 0 \\
\implies (x^2 - 1)y_{n+2} + [2(n+1)x]y_{n+1} + (n^2 - m^2)y_n &= 0
\end{aligned}$$

Hence Proved

Practice Examples

(A) Find n^{th} derivatives of following functions

1) $y = e^x$

2) $y = a^x$

(B) Find n^{th} derivatives of following functions

1) $y = \frac{8x}{x^3 - 2x^2 - 4x + 8}$

2) $y = \frac{x^3}{x^2 - 1}$

3) $y = \frac{1}{1 + x + x^2 + x^3}$

4) $y = \frac{x^3}{(x + 1)(x - 2)}$

5) $y = \frac{2x + 3}{(x - 1)(x - 2)}$

(C) Find n^{th} derivatives of following functions

1) $y = \sin 2x \sin 3x \cos 4x$

2) $y = 2^x \sin^3 x \cos^2 x$

3) $y = x \log(1 - x)$

4) $y = e^{2x} \cos x \sin^2 2x$

5) $y = e^{2x} \cos \frac{x}{2} \sin \frac{x}{2} \sin 3x$

6) $y = 2^x \cos 9x$

(D) If $y = \sin rx + \cos rx$ then prove that

$$y_n = r^n [1 + (-1)^n \sin 2rx]^{\frac{1}{2}}$$

Also find $y_8(\pi)$ where $r = \frac{1}{4}$

(E) If $y = \tan^{-1} \left(\frac{1+x}{1-x} \right)$ then prove that

$$y_n = (-1)^{n-1} (n-1)! \sin^n \theta \sin n\theta$$

where $\theta = \tan^{-1} \left(\frac{1}{x} \right)$

(F) If $y = \frac{x}{x^2 + a^2}$ then prove that

$$y_n = \frac{(-1)^n n!}{a^{n+1}} \sin^{n+1} \theta \cos(n+1)\theta$$

(G) Using Leibnitz's Theorem Find n^{th} derivatives of following functions

1) $y = x^3 \cos x$

2) $y = x^2 e^x \cos x$

3) $y = x \log(x+1)$

(H) Using Leibnitz's Theorem, Prove the following results for given functions

1) $y = x^n \log x$ then

$$y_{n+1} = \frac{n!}{x}$$

2) $y = \sin[\log(x^2 + 2x + 1)]$ then

$$(x + 1)^2 y_{n+2} + (2n + 1)(x + 1)y_{n+1} + (n^2 + 4)y_n = 0$$

3) $y = \cos^{-1} x$ then

$$(1 - x^2)y_{n+2} - (2n + 1)xy_{n+1} - n^2 y_n = 0$$

4) $\cos^{-1} \left(\frac{y}{b} \right) = \log \left(\frac{x}{n} \right)^n$ then

$$x^2 y_{n+2} + (2n + 1)xy_{n+1} + 2n^2 y_n = 0$$

5) $y = (\sin^{-1} x)^2$ then

$$(1 - x^2)y_{n+2} - (2n + 1)xy_{n+1} - n^2 y_n = 0$$

Hence find value of $y_n(0)$